examples/IOCO_ex.v
@@ -72,187 +72,143 @@ Proof.
   reflexivity.
 Qed.
 
-Lemma s1_traces :
-  forall (t : list s_label) (P : Prop),
-    (ind_s_traces_LTS t (create_s_IOLTS spec_s1_IOLTS) -> P)
-    <-> 
-    (t = [] \/ t = [s_event "a"] \/ t = [s_event "a" ; s_event "x"] -> P).
-Proof.
-  intros t P. split.
-  - intros H1 H2. apply H1.
-    unfold ind_s_traces_LTS. simpl.
-    unfold ind_s_traces.
-    destruct H2 as [H2 | [H2 | H2]].
-    -- rewrite H2. exists 1.
-       apply s_seq_reachability_r1.
-       apply empty_reachability_r1.
-    -- rewrite H2. exists 2.
-       apply s_seq_reachability_r2 with (si := 2).
-       --- apply one_step_reachability_r1 with (s1 := 1) (s2 := 2).
-           ---- apply empty_reachability_r1.
-           ---- apply transition_r1. simpl. left. reflexivity.
-           ---- apply empty_reachability_r1.
-       --- apply s_seq_reachability_r1. 
-           apply empty_reachability_r1.
-    -- rewrite H2. exists 3.
-       apply s_seq_reachability_r2 with (si := 2).
-       --- apply one_step_reachability_r1 with (s1 := 1) (s2 := 2).
-           ---- apply empty_reachability_r1.
-           ---- apply transition_r1. simpl. left. reflexivity.
-           ---- apply empty_reachability_r1.
-       --- apply s_seq_reachability_r2 with (si := 3).
-           ---- apply one_step_reachability_r1 with (s1 := 2) (s2 := 3).
-                ----- apply empty_reachability_r1.
-                ----- apply transition_r1. simpl. right. left. reflexivity.
-                ----- apply empty_reachability_r1.
-           ---- apply s_seq_reachability_r1.
-                apply empty_reachability_r1.
-  - admit.
-Admitted.
-
-(* TODO: adjust to Q1 [=] Q2 and move to /src *)
-Lemma ind_s_after_IOLTS_deterministic :
-  forall (t : list s_label) (s : s_IOLTS) (Q1 Q2 : set state),
-    ind_s_after_IOLTS t Q1 s ->
-    ind_s_after_IOLTS t Q2 s ->
-    Q1 = Q2.
-Proof.
-Admitted.
-
-Lemma i1_states_after_empty_aux :
-  ind_s_after_IOLTS [] [1] (create_s_IOLTS (embedded_iolts imp_i1)).
-Proof.
-  unfold ind_s_after_IOLTS. simpl. unfold ind_s_after. intros. split.
-  - intros H. inversion H. subst. simpl in H0.
-    inversion H0 ; subst.
-    -- simpl. left. reflexivity.
-    -- inversion H1. subst. simpl in H3.
-       repeat (destruct H3 ; inversion H3).
-  - intros H. simpl in H. destruct H as [H | H].
-    -- subst. apply s_seq_reachability_r1. simpl.
-       apply empty_reachability_r1.
-    -- contradiction.
-Qed.
-
-Lemma i1_states_after_empty :
-  forall (Q : set state),
-    ind_s_after_IOLTS [] Q (create_s_IOLTS (embedded_iolts imp_i1))
-    -> Q = [1].
-Proof.
-  intros Q. intros H1. simpl in H1.
-  pose proof (i1_states_after_empty_aux) as H2.
-  simpl in H2.
-  pose proof (
-    ind_s_after_IOLTS_deterministic
-      []
-      (create_s_IOLTS imp_i1_IOLTS)
-      Q
-      [1]
-      H1
-      H2
-  ) as H3.
-  apply H3. 
-Qed.
-
-Lemma s1_states_after_empty :
-  forall (Q : set state),
-    ind_s_after_IOLTS [] Q (create_s_IOLTS spec_s1_IOLTS)
-    -> Q = [1].
-Proof.
-Admitted.
-
-Lemma i1_out_empty :
-  forall (out : set s_label),
-    ind_out [1] out (create_s_IOLTS (embedded_iolts imp_i1))
-    -> out = [delta].
-Proof.
-Admitted.
-
-Lemma s1_out_empty :
-  forall (out : set s_label),
-    ind_out [1] out (create_s_IOLTS spec_s1_IOLTS)
-    -> out = [delta].
-Proof.
-Admitted.
-
 Example i1_ioco_s1 : ind_ioco imp_i1 spec_s1_IOLTS.
 Proof.
-  unfold ind_ioco. intros Qi Qs t out_i out_s H.
-  generalize dependent Qi.
-  generalize dependent Qs.  
-  generalize dependent out_i.
-  generalize dependent out_s.
-  generalize dependent H.
-  rewrite s1_traces. intros H.
-  intros out_s out_i Qs Qi.
-  destruct H as [H | [H | H]] ; rewrite H ; intros H1 H2 H3 H4.
-  - apply i1_states_after_empty in H1.
-    apply s1_states_after_empty in H2.
-    subst.
-    apply i1_out_empty in H3.
-    apply s1_out_empty in H4.
-    subst. unfold incl.
-    intros a H.
-    apply H.
-  - admit.
-  - admit.
-Admitted.
+  unfold ind_ioco. intros Qi Qs t out_i out_s H H1 H2 H3 H4 x H5.
+  unfold ind_s_traces_LTS in H. unfold ind_s_traces in H.
+  simpl in H. destruct H as [s H].
+  unfold ind_out in H3. destruct H3 as [H3 _].
+  unfold ind_out in H4. destruct H4 as [_ H4].
+  apply H3 in H5. destruct H5 as [s' [so' [H5_1 [H5_2 H5_3]]]].
+  unfold ind_s_after_IOLTS in H1. simpl in H1. unfold ind_s_after in H1.
+  apply H1 in H5_1.
+  unfold ind_s_after_IOLTS in H2. simpl in H2. unfold ind_s_after in H2.
+  remember H as H'. clear HeqH'. apply H2 in H'. apply H4 in H'.
+  destruct H' as [so'' [H' H'_2]]. apply H'_2.
+  clear H1 H2 H3 H4 H'_2 Qi Qs out_i out_s.
+  induction t as [| a t' IHt']; [| destruct a].
+  - (* t = [] *)
+    expand_s_seq_reachability H5_1. expand_out_one_state H5_2 x H5_3.
+    expand_s_seq_reachability H. inversion H'; [elem_in_list |].
+    destruct H1. elem_in_list.
+  - (* t = s_event "a" :: t' => destruct t' *)
+    clear IHt'. destruct t' as [| a t'']; [| destruct a].
+    + (* t = [ s_event "a" ] *)
+      expand_s_seq_reachability H.
+      expand_s_seq_reachability H5_1. expand_out_one_state H5_2 x H5_3.
+      clear H_so H5_1 H5_2 H0 H1 H4. inversion H'; [expand_In H0 |].
+      apply H2. exists 3. split; try apply transition_r1; elem_in_list.
+    + (* t = s_event "a" :: s_event "x" :: t'' => induction t'' *)
+      induction t'' as [| a t''' IHt''']; [| destruct a].
+      * (* t = [ s_event "a"; s_event "x" ] *)
+        expand_s_seq_reachability H.
+        expand_s_seq_reachability H5_1; expand_out_one_state H5_2 x H5_3.
+        clear H0 H1 H2 H3 H4. inversion H'; [elem_in_list |].
+        destruct H0. elem_in_list.
+      * (* t = s_event _ :: s_event _ :: s_event _ :: t'' => contradiction *)
+        expand_s_seq_reachability H.
+      * (* t = s_event "a" :: s_event "x" :: delta :: t''' => use IHt''' *)
+        apply IHt'''.
+        -- inversion H. subst. expand_one_step_reachability H3.
+           apply s_seq_reachability_r2 with (si := 2); auto.
+           inversion H6. subst. expand_one_step_reachability H5.
+           apply s_seq_reachability_r2 with (si := 3); auto.
+           inversion H9. subst. apply H8.
+        -- inversion H5_1. subst. expand_one_step_reachability H3;
+           eapply s_seq_reachability_r2; try (apply H3);
+           inversion H6; subst; expand_one_step_reachability H5;
+           eapply s_seq_reachability_r2; try (apply H5); inversion H9; auto.
+    + (* t = s_event "a" :: delta :: t'' => contradiction *)
+      expand_s_seq_reachability H.
+  - (* t = delta :: t' => use IHt' *)
+    inversion H5_1. subst. inversion H. subst. apply IHt'; auto.
+Qed.
 
-(*
-  unfold ind_ioco. intros Qi Qs t out_i out_s H H1 H2 H3 H4.
-  apply ind_out_equiv_f_out in H3. simpl in H3.
-  apply ind_out_equiv_f_out in H4. simpl in H4.
-  unfold incl. intros l H5. apply H3 in H5. apply H4.
-  clear H1.
-  assert (H1 : Qi [=] (f_after_IOLTS t (create_s_IOLTS (embedded_iolts imp_i1)))).
-  { admit. }
-  clear H2.
-  assert (H2 : Qs [=] (f_after_IOLTS t (create_s_IOLTS spec_s1_IOLTS))).
-  { admit. }
-  clear H3 H4.
-  induction H. simpl in H. induction t.
-  - simpl in H. unfold f_after_IOLTS in H2. unfold f_after_single_state_IOLTS in H2.
-    simpl in H2. unfold LTS_functions.all_reachable_by_tau in H2. simpl in H2.  admit.
-  - 
-  unfold incl. intros l' H'.
-  unfold ind_out in H3. specialize (H3 l'). destruct H3 as [H3_1 H3_2].
-  unfold ind_out in H4. specialize (H4 l'). destruct H4 as [H4_1 H4_2].
-  apply H3_1 in H'. destruct H' as [s'' [so [H'_1 [H'_2 H'_3]]]].
-  inversion H'_2; subst.
-  + expand_In H'_3; subst. expand_In H3; subst.
-    * unfold ind_s_after_LTS in H1. unfold ind_s_after in H1. simpl in *.
-      unfold ind_s_after_LTS in H2. unfold ind_s_after in H2. simpl in H2.
-      apply H1 in H'_1. inversion H'_1; subst.
-      * simpl in H0. unfold ind_s_traces_LTS in H.
-        unfold ind_s_traces in H. destruct H as [s'' H]. simpl in H. inversion H; subst.
-        simpl in *. inversion H5; subst.
-        -- apply H2 in H. apply H4_2 in H. destruct H as [so' [H_1 H_2]].
-           inversion H_1; subst.
-           ++ apply H_2. elem_in_list.
-           ++ destruct H. elem_in_list.
-        -- inversion H6; subst. expand_In H8.
-      * simpl in *. inversion H0; subst. inversion H6; subst.
-        -- inversion H7; subst. expand_In H11; subst.
-    unfold ind_out in H4. specialize (H4 l). destruct H4 as [H4_1 H4_2].
-    
-  
-  
-   inversion H0; subst.
-    + intros H1 H2 H3 H4. unfold ind_s_after_LTS in H2. unfold ind_s_after in H2.
-      simpl in H2. apply H2 in H. 
-      apply H4_2 in H. destruct H as [so' [H_1 H_2]]. inversion H_1; subst.
-      * apply H_2. apply H3_1 in H''.
-    intros H'. unfold ind_s_after_LTS in H'. unfold ind_s_after in H'.
-    simpl in *. intros H1 H2 H3.  
-    unfold ind_out in H2. specialize (H2 l). destruct H2 as [H2_1 H2_2].
-    unfold ind_out in H3. specialize (H3 l). destruct H3 as [H3_1 H3_2].
-    apply H2_1 in H''.
-    destruct H'' as [s [so' [H''_1 [H''_2 H''_3]]]]. inversion H''_2; subst.
-    + expand_In H''_3; subst. unfold ind_s_after_LTS in H1. unfold ind_s_after in H1.
-      simpl in *. 
-      *
-Admitted.
-*)
+(* "mais correto"
+  unfold ind_ioco. intros Qi Qs t out_i out_s H H1 H2 H3 H4 x H5.
+  unfold ind_s_traces_LTS in H. unfold ind_s_traces in H.
+  simpl in H. destruct H as [s H].
+  unfold ind_out in H3. destruct H3 as [H3 _].
+  unfold ind_out in H4. destruct H4 as [_ H4].
+  apply H3 in H5. destruct H5 as [s' [so' [H5_1 [H5_2 H5_3]]]].
+  unfold ind_s_after_IOLTS in H1. simpl in H1. unfold ind_s_after in H1.
+  apply H1 in H5_1.
+  assert(H': forall s : state,
+    ind_s_seq_reachability 1 t s (create_s_IOLTS spec_s1_IOLTS) ->
+    exists so' : set s_label,
+       ind_out_one_state s so' (create_s_IOLTS spec_s1_IOLTS) /\
+       (forall o : s_label, In o so' -> In o out_s)).
+  { intros s'' H''. apply H4. apply H2. apply H''. }
+  clear H1 H2 H3 H4.
+  induction t as [| a t' IHt']; [| destruct a].
+  - (* t = [] *)
+    expand_s_seq_reachability H5_1; expand_out_one_state H5_2 x H5_3. clear H.
+    assert (H: ind_s_seq_reachability 1 [] 1 (create_s_IOLTS spec_s1_IOLTS)).
+    { apply s_seq_reachability_r1. apply empty_reachability_r1. }
+    apply H' in H.
+    destruct H as [so [H_1 H_2]]. apply H_2. inversion H_1; [elem_in_list |].
+    destruct H. elem_in_list.
+  - (* t = s_event "a" :: t' => destruct t' *)
+    clear IHt'. destruct t' as [| a t'']; [| destruct a].
+    + (* t = [ s_event "a" ] *)
+      expand_s_seq_reachability H.
+      expand_s_seq_reachability H5_1; expand_out_one_state H5_2 x H5_3.
+      clear H_so H5_1 H5_2 H H0 H1 H4.
+      assert (H: ind_s_seq_reachability 1 [s_event "a"] 2 (create_s_IOLTS spec_s1_IOLTS)).
+      { eapply s_seq_reachability_r2.
+        - apply one_step_reachability_r1 with (s1 := 1) (s2 := 2);
+          try apply empty_reachability_r1. apply transition_r1. elem_in_list.
+        - apply s_seq_reachability_r1. apply empty_reachability_r1. }
+      apply H' in H.
+      destruct H as [so [H_1 H_2]]. apply H_2. inversion H_1; [ expand_In H |].
+      apply H1. exists 3. split; try apply transition_r1; elem_in_list.
+    + (* t = s_event "a" :: s_event "x" :: t'' => induction t'' *)
+      induction t'' as [| a t''' IHt''']; [| destruct a].
+      * (* t = [ s_event "a"; s_event "x" ] *)
+        expand_s_seq_reachability H.
+        expand_s_seq_reachability H5_1; expand_out_one_state H5_2 x H5_3.
+        clear H H0 H1 H2 H3 H4.
+        assert (H:
+          ind_s_seq_reachability
+            1
+            [s_event "a"; s_event "x"]
+            3
+            (create_s_IOLTS spec_s1_IOLTS)).
+        { eapply s_seq_reachability_r2.
+          - apply one_step_reachability_r1 with (s1 := 1) (s2 := 2);
+            try apply empty_reachability_r1. apply transition_r1. elem_in_list.
+          - eapply s_seq_reachability_r2.
+            + apply one_step_reachability_r1 with (s1 := 2) (s2 := 3);
+              try apply empty_reachability_r1. apply transition_r1. elem_in_list.
+            + apply s_seq_reachability_r1. apply empty_reachability_r1. }
+        apply H' in H.
+        destruct H as [so [H_1 H_2]]. apply H_2. inversion H_1; [elem_in_list |].
+        destruct H. elem_in_list.
+      * (* t = s_event _ :: s_event _ :: s_event _ :: t'' => contradiction *)
+        expand_s_seq_reachability H.
+      * (* t = s_event "a" :: s_event "x" :: delta :: t''' => use IHt''' *)
+        apply IHt'''.
+        -- inversion H. subst. expand_one_step_reachability H3.
+           apply s_seq_reachability_r2 with (si := 2); auto.
+           inversion H6. subst. expand_one_step_reachability H5.
+           apply s_seq_reachability_r2 with (si := 3); auto.
+           inversion H9. subst. apply H8.
+        -- inversion H5_1. subst. expand_one_step_reachability H3;
+           eapply s_seq_reachability_r2; try (apply H3);
+           inversion H6; subst; expand_one_step_reachability H5;
+           eapply s_seq_reachability_r2; try (apply H5); inversion H9; auto.
+        -- intros s'' H''. apply H'. inversion H''.
+           subst. expand_one_step_reachability H3.
+           apply s_seq_reachability_r2 with (si := 2); auto.
+           inversion H6. subst. expand_one_step_reachability H5.
+           apply s_seq_reachability_r2 with (si := 3); auto.
+           apply s_seq_reachability_r3; auto. elem_in_list.
+    + (* t = s_event "a" :: delta :: t'' => contradiction *)
+      expand_s_seq_reachability H.
+  - (* t = delta :: t' => use IHt' *)
+    inversion H5_1. subst. inversion H. subst. apply IHt'; auto.
+    intros s'' H''. apply H'. apply s_seq_reachability_r3; auto.
+Qed. *)
 
 Example i1_not_ioco_s3 : ~ (ind_ioco imp_i1 spec_s3_IOLTS).
 Proof.
@@ -265,10 +221,11 @@ Proof.
   apply H'. apply H.
   - unfold ind_s_traces_LTS. unfold ind_s_traces. exists 4. simpl.
     apply s_seq_reachability_r2 with (si := 4).
-    + apply one_step_reachability_r1 with (s1 := 1) (s2 := 4); try apply empty_reachability_r1.
+    + apply one_step_reachability_r1 with (s1 := 1) (s2 := 4);
+      try apply empty_reachability_r1.
       apply transition_r1. elem_in_list.
     + apply s_seq_reachability_r1. apply empty_reachability_r1.
-  - unfold ind_s_after_LTS. unfold ind_s_after. intros a. split.
+  - unfold ind_s_after_IOLTS. unfold ind_s_after. intros a. split.
     + simpl. intros H''. inversion H''; subst. simpl in *. inversion H3; subst.
       inversion H0; subst.
       * inversion H1; subst. expand_In H7. subst. inversion H2; subst.
@@ -278,10 +235,11 @@ Proof.
         -- inversion H4; subst. expand_In H8.
       * inversion H4; subst. expand_In H7.
     + intros H''. expand_In H''. simpl. apply s_seq_reachability_r2 with (si := 1).
-      * apply one_step_reachability_r1 with (s1 := 1) (s2 := 1); try apply empty_reachability_r1.
+      * apply one_step_reachability_r1 with (s1 := 1) (s2 := 1);
+        try apply empty_reachability_r1.
         apply transition_r1. elem_in_list.
       * apply s_seq_reachability_r1. apply empty_reachability_r1.
-  - unfold ind_s_after_LTS. unfold ind_s_after. intros a. split.
+  - unfold ind_s_after_IOLTS. unfold ind_s_after. intros a. split.
     + simpl. intros H''. inversion H''; subst. simpl in *. inversion H3; subst.
       inversion H0; subst.
       * inversion H1; subst. expand_In H7. subst. inversion H2; subst.
@@ -291,24 +249,26 @@ Proof.
         -- inversion H4; subst. expand_In H8.
       * inversion H4; subst. expand_In H7.
     + intros H''. expand_In H''. simpl. apply s_seq_reachability_r2 with (si := 4).
-      * apply one_step_reachability_r1 with (s1 := 1) (s2 := 4); try apply empty_reachability_r1.
+      * apply one_step_reachability_r1 with (s1 := 1) (s2 := 4);
+        try apply empty_reachability_r1.
         apply transition_r1. elem_in_list.
       * apply s_seq_reachability_r1. apply empty_reachability_r1.
-  - unfold ind_out. intros l. split.
-    + intros H''. expand_In H''. exists 1. exists [delta].
+  - unfold ind_out. split.
+    + intros l H''. expand_In H''. exists 1. exists [delta].
       repeat split; try(apply out_one_state_r1); elem_in_list.
     + intros s H''. expand_In H''. exists [delta]. split.
       * try(apply out_one_state_r1); elem_in_list.
       * intros o H'''. expand_In H'''. elem_in_list.
-  - unfold ind_out. intros l. split.
-    + intros H''. expand_In H''. exists 4. exists [s_event "y"].
+  - unfold ind_out. split.
+    + intros l H''. expand_In H''. exists 4. exists [s_event "y"].
       repeat split; try elem_in_list. apply out_one_state_r2.
       * intros H'''; expand_In H'''.
       * intros H'''; expand_In H'''.
       * intros l'. split.
         -- intros H'''. expand_In H'''. exists 5. split; try (elem_in_list).
            apply transition_r1. elem_in_list.
-        -- intros H'''. destruct H''' as [ s' [ H'''_1 H'''_2]]. inversion H'''_2; subst.
+        -- intros H'''. destruct H''' as [ s' [ H'''_1 H'''_2]].
+           inversion H'''_2; subst.
            expand_In H'''_1; subst; expand_In H3. elem_in_list.
     + intros s H''. expand_In H''. exists [s_event "y"]. split.
       * apply out_one_state_r2.
@@ -316,8 +276,9 @@ Proof.
         -- intros H'''; expand_In H'''.
         -- intros l'. split.
            ++ intros H'''. expand_In H'''. exists 5. split; try (elem_in_list).
-           apply transition_r1. elem_in_list.
-           ++ intros H'''. destruct H''' as [ s' [ H'''_1 H'''_2]]. inversion H'''_2; subst.
-           expand_In H'''_1; subst; expand_In H3. elem_in_list.
+              apply transition_r1. elem_in_list.
+           ++ intros H'''. destruct H''' as [ s' [ H'''_1 H'''_2]].
+              inversion H'''_2; subst. expand_In H'''_1; subst; expand_In H3.
+              elem_in_list.
       * intros l' H'''. expand_In H'''. elem_in_list.
 Qed.
